proof/old_system/uni/def_extra.v
@@ -1,10 +1,32 @@
+Require Import Metalib.Metatheory.
+Require Import List.
+
 Require Import uni.def_ott.
 
-Inductive work : Set := 
+
+Fixpoint ftvar_in_aworklist' (aW_5:aworklist) : vars :=
+  match aW_5 with
+  | aworklist_empty => empty
+  | (aworklist_consvar aW x ab) => (ftvar_in_aworklist' aW) \u (ftvar_in_abind ab)
+  | (aworklist_constvar aW X ab) => (ftvar_in_aworklist' aW) \u (ftvar_in_abind ab) \u (singleton X)
+  | (aworklist_conswork aW w) => (ftvar_in_aworklist' aW) \u (ftvar_in_work w)
+end.
+
+
+Fixpoint fvar_in_aworklist' (aW_5:aworklist) : vars :=
+  match aW_5 with
+  | aworklist_empty => {}
+  | (aworklist_consvar aW x ab) => (fvar_in_aworklist' aW) \u (singleton x) (* no var in abind *)
+  | (aworklist_constvar aW X ab) => (fvar_in_aworklist' aW) (* no var in abind *)
+  | (aworklist_conswork aW w) => (fvar_in_aworklist' aW) \u (fvar_in_work w)
+end.
+  
+
+(* Inductive work : Set := 
  | work_infer (e:exp) (c:typ -> work)
  | work_check (e:exp) (A:typ)
  | work_infabs (A:typ) (c:typ -> work)
  | work_infapp (A:typ) (e:exp) (c:typ -> work)
  | work_inftapp (A1:typ) (A2:typ) (c:typ -> work)
  | work_sub (A1:typ) (A2:typ)
- | work_apply (c:typ -> work) (A:typ).
+ | work_apply (c:typ -> work) (A:typ). *)
